Fix Renest.

Renest.v
@@ -1,4 +1,4 @@
-Require Import paco2 AllInRel Util Map Env EnvTy Exp IL Sim DecSolve MoreList Sawtooth InRel Sublist.
+Require Import paco2 AllInRel Util Map Env EnvTy Exp IL SimI DecSolve MoreList Sawtooth InRel Sublist.
 
 Set Implicit Arguments.
 Unset Printing Records.
@@ -77,21 +77,6 @@ Proof.
       inv H; eauto.
 Qed.
 
-Lemma mapi_app X Y (f:nat -> X -> Y) n L L'
-: mapi_impl f n (L++L') = mapi_impl f n L ++ mapi_impl f (n+length L) L'.
-Proof.
-  general induction L; simpl; eauto.
-  - orewrite (n + 0 = n); eauto.
-  - f_equal. rewrite IHL. f_equal; f_equal. omega.
-Qed.
-
-Lemma drop_app_eq X (L L' : list X) n
-: length L = n
-  -> drop n (L ++ L') = L'.
-Proof.
-  intros; subst. orewrite (length L = length L + 0) . eapply drop_app.
-Qed.
-
 Lemma egalize_funs_get2 D n' F L' f Zb sb
   : get F f (Zb, sb)
     -> exists L'',
@@ -120,13 +105,6 @@ Proof.
     eapply H0.
 Qed.
 
-Lemma app_drop X (L L' L'':list X)
- : L = L' ++ L''
-   -> drop (length L') L = L''.
-Proof.
-  general induction L'; simpl; eauto.
-Qed.
-
 Ltac simpl_get_dropI :=
   repeat match goal with
   | [ H : get (drop (?n - _) ?L) _ _, H' : get ?L ?n ?blk, STL: sawtooth ?L |- _ ]
@@ -141,76 +119,12 @@ Ltac simpl_get_dropI :=
         orewrite (n - I.block_n blk + I.block_n blk = n); clear X
   end.
 
-Lemma sawtooth_app B `{BlockType B} L L'
-  : sawtooth L -> sawtooth L' -> sawtooth (L ++ L').
-Proof.
-  intros H1 H2. general induction H1; eauto.
-  rewrite <- app_assoc. econstructor; eauto.
-Qed.
-
 Ltac not_activated H :=
   let STEP := fresh "STEP" in
   destruct H as [? [? STEP]]; inv STEP.
 
 Ltac not_normal H :=
   destruct H; econstructor; eexists; econstructor; eauto.
-
-Lemma bisim_drop_shift_left r l (L:I.labenv) E Y
-      blk (STL:sawtooth L) sigma
-  : get L (labN l) blk
-    -> paco3 (@sim_gen I.state _ I.state _) r
-            (drop (labN l - block_n blk) L, E, stmtApp (LabI (block_n blk)) Y)
-            sigma
-    -> paco3 (@sim_gen I.state _ I.state _) r
-            (L, E, stmtApp l Y)
-            sigma.
-Proof.
-  intros GetL SIM. pinversion SIM; subst.
-  - eapply plus2_destr_nil in H. destruct H as [? [? ?]].
-    invt step. clear H. simpl in *.
-    eapply get_drop in Ldef. exploit (sawtooth_smaller STL GetL); eauto.
-    simpl in *.
-    assert (l_eq:labN l - I.block_n blk + I.block_n blk = labN l). omega.
-    rewrite l_eq in *. get_functional.
-    orewrite (I.block_n blk - I.block_n blk = 0) in H2. simpl in *.
-    pfold.
-    econstructor 1.
-    eapply star2_plus2. econstructor; eauto. eapply H2. eauto. eauto.
-  - inv H.
-    + exfalso. not_activated H1.
-    + invt step. clear H6. simpl in *.
-      eapply get_drop in Ldef. exploit (sawtooth_smaller STL GetL); eauto.
-      simpl in *.
-      assert (l_eq:labN l - I.block_n blk + I.block_n blk = labN l). omega.
-      rewrite l_eq in *. get_functional. subst.
-      orewrite (I.block_n blk - I.block_n blk = 0) in H8. simpl in *.
-      pfold.
-      econstructor 2.
-      eapply star2_silent. econstructor; eauto. eapply H8. eauto. eauto. eauto.
-      eauto. eauto.
-  - inv H0.
-    + assert ( get (drop (labN l - block_n blk) L) (counted (LabI (block_n blk))) blk). {
-        eapply drop_get. simpl.
-        exploit (sawtooth_smaller STL); eauto. simpl in *.
-        orewrite (labN l - I.block_n blk + I.block_n blk = labN l). eauto.
-      }
-      decide (❬I.block_Z blk❭ = ❬Y❭).
-      case_eq (omap (exp_eval E) Y); intros.
-      not_normal H2.
-      pfold. econstructor 3. Focus 2. eapply star2_refl. eauto. eauto.
-      stuck2. eauto.
-      pfold. econstructor 3. Focus 2. eapply star2_refl. eauto. eauto.
-      stuck2. eauto.
-    + invt step. clear H5. simpl in *.
-      eapply get_drop in Ldef. exploit (sawtooth_smaller STL GetL); eauto.
-      simpl in *.
-      assert (l_eq:labN l - I.block_n blk + I.block_n blk = labN l). omega.
-      rewrite l_eq in *. get_functional. subst.
-      orewrite (I.block_n blk - I.block_n blk = 0) in H7. simpl in *.
-      pfold. econstructor 3. Focus 2.
-      eapply star2_silent. econstructor; eauto. eapply H7. eauto. eauto. eauto.
-      eauto.
-Qed.
 
 
 (* A proof relation is parameterized by analysis information A *)
@@ -226,163 +140,147 @@ Class ProofRelationI (A:Type) := {
     IndexRelI : 〔A〕 -> nat -> nat -> Prop;
     ArgLengthMatchI : forall E E' a Z Z' VL VL',
         ParamRelI a Z Z' -> ArgRelI E E' a VL VL' -> length Z = length VL /\ length Z' = length VL';
-    IndexRelDrop : forall k AL n n', IndexRelI AL n n' -> k <= n -> IndexRelI (drop k AL) (n - k) n'
+    IndexRelDrop : forall AL' AL n n', IndexRelI (AL' ++ AL) n n' ->
+                                  n >= length AL'
+                                  -> IndexRelI AL (n - length AL') (n')
 (*    IndexRelApp : forall AL AL' n n', IndexRelI AL n n' -> IndexRelI (AL' ++ AL) (❬AL'❭ + n) n' *)
 }.
 
-Inductive simIBlock (SIM:ProgramEquivalence I.state I.state)
-          (r:I.state -> I.state -> Prop)
-          {A} (AR:ProofRelationI A)
-  : list A -> I.labenv -> I.labenv -> A -> I.block -> I.block -> Prop :=
-| simIBlockI a L L' Z Z' s s' n n' bn' AL
-  : ParamRelI a Z Z'
-    -> BlockRelI a (I.blockI Z s n) (I.blockI Z' s' bn')
-    -> IndexRelI AL n n'
-    -> (forall E E' Yv Y'v Y Y',
-          omap (exp_eval E) Y = Some Yv
-          -> omap (exp_eval E') Y' = Some Y'v
-          -> ArgRelI E E' a Yv Y'v
-          -> progeq r (L, E, stmtApp (LabI n) Y)
-                   (L', E', stmtApp (LabI n') Y'))
-          -> simIBlock SIM r AR AL L L' a (I.blockI Z s n) (I.blockI Z' s' bn').
+Definition irel := rel3 simtype (fun _ : simtype => I.state)
+                       (fun (_ : simtype) (_ : I.state) => I.state).
 
 
-Definition renILabenv (SIM:ProgramEquivalence I.state I.state) r
-           {A} AR (AL:list A) L L' :=
+Definition simILabenv t (r:irel)
+           {A} (PR:ProofRelationI A) (AL:list A) L L' :=
   (length AL = length L /\ tooth 0 L' /\ sawtooth L) /\
-  forall n n' a b b', IndexRelI AL n n' -> get AL n a -> get L n b -> get L' n' b'
-               -> simIBlock SIM r AR
-                           (drop (n - I.block_n b) AL)
-                           (drop (n - I.block_n b) L)
-                           L'
-                           a b b' .
+  forall f f' a Z s n Z' s' n',
+    IndexRelI AL (counted f) (counted f')
+    -> get AL (counted f) a
+    -> get L (counted f) (I.blockI Z s n)
+    -> get L' (counted f') (I.blockI Z' s' n')
+    -> (ParamRelI a Z Z' /\ BlockRelI a (I.blockI Z s n) (I.blockI Z' s' n'))
+      /\ (forall E E' Yv Y'v Y Y',
+            ArgRelI E E' a Yv Y'v
+            -> omap (exp_eval E) Y = Some Yv
+            -> omap (exp_eval E') Y' = Some Y'v
+            -> sim'r r t (L, E, stmtApp f Y)
+                    (L', E', stmtApp f' Y')).
 
-Definition fexteqI (SIM:ProgramEquivalence I.state I.state)
-           {A} (PR:ProofRelationI A) (a:A) (AL:list A) L L' Z s Z' s' :=
-  ParamRelI a Z Z' /\
-  forall E E' VL VL' (r:rel2 I.state (fun _ : I.state => I.state)),
-    ArgRelI E E' a VL VL'
-    -> renILabenv SIM r PR AL L L'
-    -> progeq r (L, E[Z <-- List.map Some VL], s)
+Lemma simILabenv_mon t (r r':irel) A (PR:ProofRelationI A) AL L L'
+  : simILabenv t r PR AL L L'
+    -> (forall t x y, r t x y -> r' t x y)
+    -> simILabenv t r' PR AL L L'.
+Proof.
+  intros [[? ?] SIM] LE; hnf; intros; split; eauto.
+  intros. edestruct SIM as [[? ?] SIM']; eauto.
+  split; eauto. intros.
+  eapply paco3_mon. eapply SIM; eauto. eauto.
+Qed.
+
+Definition indexwise_r t (r:irel) A (PR:ProofRelationI A) AL' F AL L L' :=
+  forall n n' Z s Z' s' a i,
+    IndexRelI (AL' ++ AL) n n'
+    -> get F n (Z,s)
+    -> get L' n' (I.blockI Z' s' i)
+    -> get AL' n a
+    -> forall E E' VL VL',
+        ArgRelI E E' a VL VL'
+        -> r t (mapi I.mkBlock F ++ L, E[Z <-- List.map Some VL], s)
             (L', E'[Z' <-- List.map Some VL'], s').
 
-Lemma fix_compatible_I r A (PR:ProofRelationI A) (a:A) AL F E E' Z Z' L L' Yv Y'v s s' n n' AL' bn
-(LEN2:length AL' = length F)
-  : renILabenv bisim_progeq r PR AL L L'
-    -> (forall n n' Z s Z' s' a bn, get F n (Z,s) -> IndexRelI (AL' ++ AL) n n'
-                              -> get L' n' (I.blockI Z' s' bn) -> get AL' n a ->
-                             fexteqI bisim_progeq PR a (AL' ++ AL) (mapi I.mkBlock F ++ L) L' Z s Z' s'
-                             /\ BlockRelI a (I.blockI Z s n) (I.blockI Z' s' bn)
-                             /\ ParamRelI a Z Z')
-    -> get F n (Z,s)
-    -> IndexRelI (AL' ++ AL) n n'
-    -> get L' n' (I.blockI Z' s' bn)
-    -> get AL' n a
-    -> ArgRelI E E' a Yv Y'v
-    -> tooth 0 L'
-    -> sawtooth L
-    -> bisim'r r
-              (mapi I.mkBlock F ++ L, E [Z <-- List.map Some Yv], s)
-              (L', E' [Z' <-- List.map Some Y'v], s').
+Lemma indexwise_r_mon t (r r':irel) A (PR:ProofRelationI A) AL' F AL L L'
+  : indexwise_r t r PR AL' F AL L L'
+    -> (forall t x y, r t x y -> r' t x y)
+    -> indexwise_r t r' PR AL' F AL L L'.
 Proof.
-  revert_all; pcofix CIH; intros.
-  eapply H1; eauto. clear H2 H3 H4 H5 H6. clear s s' Z Z' n n' a bn.
+  intros Idx LE; hnf; intros; eauto.
+Qed.
+
+Definition indexwise_proofrel A (PR:ProofRelationI A) (F:〔params * stmt〕) AL' L' AL :=
+  forall n n' Z s Z' s' a i,
+    IndexRelI (AL' ++ AL) n n'
+    -> get F n (Z,s)
+    -> get L' n' (I.blockI Z' s' i)
+    -> get AL' n a
+    -> ParamRelI a Z Z' /\ BlockRelI a (I.blockI Z s n) (I.blockI Z' s' i).
+
+Lemma simILabenv_extension' t (r:irel) A (PR:ProofRelationI A) (AL AL':list A) F L L'
+      (LEN1:length AL' = length F)
+  : indexwise_r t (sim'r r \3/ r) PR AL' F AL L L'
+    -> indexwise_proofrel PR F AL' L' AL
+    -> simILabenv t r PR AL L L'
+    -> simILabenv t r PR (AL' ++ AL) (mapi I.mkBlock F ++ L) L'.
+Proof.
+  intros ISIM IP SIML.
   hnf. split.
-  destruct H0; dcr; split; eauto with len. split; eauto.
+  destruct SIML; dcr; split; eauto with len. split; eauto.
   econstructor; eauto. eapply tooth_I_mkBlocks.
-  intros ? ? ? ? ? RN GetAL GetFL GetL'.
+  intros f f' ? ? ? ? ? ? ? RN GetAL GetFL GetL'.
   assert (❬AL'❭ = ❬mapi I.mkBlock F❭) by eauto with len.
-  eapply get_app_cases in GetAL. destruct GetAL.
+  eapply get_app_cases in GetAL. destruct GetAL as [GetAL'|GetAL].
   - eapply get_app_lt_1 in GetFL; [| rewrite <- H; eauto using get_range].
-    inv_get. destruct x as [Z s]. destruct b' as [Z' s' bn]. simpl.
-    assert (bn = n'). {
-      exploit (tooth_index H7 GetL'); eauto. simpl in *. omega.
-    }
-    subst bn.
-    orewrite (n - n = 0). simpl.
-    exploit H1; eauto; dcr.
-    eapply simIBlockI; eauto. simpl.
+    inv_get. destruct x as [Z s]. simpl in *. clear EQ.
+    split; eauto.
+    intros.
+    exploit (ArgLengthMatchI); eauto; dcr. eapply IP; eauto.
+    pone_step; eauto using get_app, get_mapi; eauto; simpl; eauto with len.
+    destruct SIML; dcr.
+    exploit (tooth_index H9 GetL'); eauto; simpl in *; subst.
+    orewrite (labN f' + 0 = labN f'); simpl.
+    orewrite (labN f - labN f = 0); simpl.
+    orewrite (labN f' - labN f' = 0); simpl.
+    eapply ISIM; eauto.
+  - destruct SIML; dcr.
+    eapply get_app_right_ge in GetFL; [ | rewrite <- H; eauto].
+    rewrite mapi_length in *.
+    eapply IndexRelDrop in RN; eauto.
+    edestruct (H1 (LabI (counted f - ❬AL'❭)) (LabI (counted f')))
+      as [[? ?] SIM]; simpl; eauto.
+    rewrite H; eauto.
+    split; eauto.
     intros.
     exploit (ArgLengthMatchI); eauto; dcr.
-    pone_step; eauto using get_app, get_mapi; simpl; eauto with len.
-    orewrite (n - n = 0); simpl.
-    right.
-    orewrite (n' - n' = 0); simpl.
-    eapply CIH; eauto.
-  - destruct H0.
-    dcr. eapply get_app_right_ge in GetFL; [ | rewrite <- H; eauto].
-    assert (n - I.block_n b >= ❬mapi I.mkBlock F❭). {
-      exploit (sawtooth_smaller H8 GetFL). rewrite <- H in *. simpl in *. omega.
-    }
-    exploit H3. instantiate (2:=n-❬mapi I.mkBlock F❭). instantiate (1:=n').
-    eapply IndexRelDrop in RN. instantiate (1:=❬AL'❭) in RN.
-    rewrite drop_length_eq in RN. rewrite <- H. eauto. omega.
-    rewrite <- H. eauto. eauto. eauto.
-    rewrite (drop_app_gen _ (mapi I.mkBlock F)); eauto.
-    assert (EQ:n - ❬mapi I.mkBlock F❭ - I.block_n b = n - I.block_n b - ❬mapi I.mkBlock F❭)
-      by omega.
-    rewrite <- EQ.
-    inv H6. econstructor; eauto. simpl in *.
-    rewrite (drop_app_gen _ AL'); eauto.
-    rewrite H. rewrite <- EQ. eauto. omega.
-    intros. eapply progeq_mon; eauto.
+    eapply (@sim_Y_left I.state _ I.state _).
+    eapply (@sim_Y_right I.state _ I.state _).
+    rewrite H in SIM.
+    eapply SIM; eauto.
+    econstructor; simpl; eauto with len. simpl. eauto with len.
+    Focus 2.
+    econstructor; simpl; eauto. simpl. eauto with len.
+    simpl.
+    eapply (I.stepGoto _ _ _ GetL'); simpl; eauto with len.
+    eapply (stepGoto_mapi _ _ _ _ GetFL); simpl; eauto with len.
+    simpl in *; omega.
 Qed.
 
+Lemma fix_compatible_I t A (PR:ProofRelationI A) AL F L L' AL'
+(LEN2:length AL' = length F)
+  : (forall r, simILabenv t r PR (AL' ++ AL) (mapi I.mkBlock F ++ L) L'
+            -> indexwise_r t (sim'r r) PR AL' F AL L L')
+    -> indexwise_proofrel PR F AL' L' AL
+    -> forall r, simILabenv t r PR AL L L'
+           -> indexwise_r t (sim'r r) PR AL' F AL L L'.
+Proof.
+  intros ISIM IP r SIML; pcofix CIH.
+  eapply ISIM; eauto.
+  hnf. split.
+  destruct SIML; dcr; split; eauto with len. split; eauto.
+  econstructor; eauto. eapply tooth_I_mkBlocks.
+  eapply simILabenv_extension'; eauto using simILabenv_mon, indexwise_r_mon.
+Qed.
 
-Lemma renILabenv_extension r A (PR:ProofRelationI A) (AL AL':list A) F L L'
+Lemma simILabenv_extension t A (PR:ProofRelationI A) (AL AL':list A) F L L'
       (LEN1:length AL' = length F)
-  : renILabenv bisim_progeq r PR AL L L'
-    -> (forall n n' Z s Z' s' a bn, get F n (Z,s) -> IndexRelI (AL' ++ AL) n n'
-                              -> get L' n' (I.blockI Z' s' bn) -> get AL' n a ->
-                              fexteqI bisim_progeq PR a (AL' ++ AL) (mapi I.mkBlock F ++ L) L' Z s Z' s'
-                              /\ BlockRelI a (I.blockI Z s n) (I.blockI Z' s' bn)
-                              /\ ParamRelI a Z Z')
-  -> renILabenv bisim_progeq r PR (AL' ++ AL) (mapi I.mkBlock F ++ L) L'.
+  : (forall r, simILabenv t r PR (AL' ++ AL) (mapi I.mkBlock F ++ L) L'
+          -> indexwise_r t (sim'r r) PR AL' F AL L L')
+    -> indexwise_proofrel PR F AL' L' AL
+    -> forall r, simILabenv t r PR AL L L'
+           -> simILabenv t r PR (AL' ++ AL) (mapi I.mkBlock F ++ L) L'.
 Proof.
-  intros. destruct H.
-  split. dcr. split. eauto with len.
-  split; eauto. econstructor; eauto using tooth_I_mkBlocks.
-  intros ? ? ? ? ? RN GetAL GetL GetL'.
-  assert (ALLEN:❬AL'❭ = ❬mapi I.mkBlock F❭) by eauto with len.
-  eapply get_app_cases in GetAL. destruct GetAL.
-  - eapply get_app_lt_1 in GetL; [| rewrite <- ALLEN; eauto using get_range].
-    inv_get. destruct x, b'.
-    exploit H0; eauto. simpl in *. dcr.
-    destruct H4. orewrite (n - n = 0); simpl.
-    econstructor; eauto. intros.
-    exploit (ArgLengthMatchI); eauto; dcr.
-    pone_step; eauto using get_app, get_mapi; simpl; eauto with len.
-    left. orewrite (n - n = 0); simpl.
-    exploit (tooth_index H8 GetL'); eauto. simpl in *.
-    orewrite (n' + 0 = n') in H12. subst; simpl in *.
-    orewrite (n' - n' = 0); simpl.
-    eapply fix_compatible_I; eauto.
-    split; eauto.
-  - dcr.
-    eapply get_app_right_ge in GetL; [ | rewrite <- ALLEN; eauto].
-    assert (n - I.block_n b >= ❬mapi I.mkBlock F❭). {
-      exploit (sawtooth_smaller H7 GetL). rewrite <- ALLEN in *. simpl in *. omega.
-    }
-    rewrite (drop_app_gen _ (mapi I.mkBlock F)); eauto.
-    rewrite (drop_app_gen _ AL'); [ | rewrite ALLEN; eauto ].
-    assert (EQ:n - ❬mapi I.mkBlock F❭ - I.block_n b = n - I.block_n b - ❬mapi I.mkBlock F❭)
-      by omega.
-    rewrite ALLEN. rewrite <- EQ.
-    eapply H1; eauto.
-    eapply IndexRelDrop in RN. instantiate (1:= ❬mapi I.mkBlock F❭) in RN.
-    rewrite <- ALLEN in RN. rewrite drop_length_eq in RN.
-    rewrite ALLEN in RN. eauto. rewrite <- ALLEN. omega.
-    rewrite <- ALLEN. eauto.
+  intros. eapply simILabenv_extension'; eauto.
+  eapply indexwise_r_mon.
+  eapply fix_compatible_I; eauto. eauto.
 Qed.
-
-Lemma nth_drop X (L:list X) n m x
-: nth n (drop m L) x = nth (n+m) L x.
-Proof.
-  general induction m; simpl. orewrite (n + 0 = n); eauto.
-  rewrite IHm; eauto. orewrite (n + S m = S (n + m)); eauto.
-  destruct L; simpl; eauto. destruct (n + m); eauto.
-Qed.
-
 Instance PR : ProofRelationI (params * nat) :=
   {
     ParamRelI G Z Z' := Z = Z' /\ fst G = Z;
@@ -395,7 +293,7 @@ Instance PR : ProofRelationI (params * nat) :=
 intros. dcr; repeat subst. eauto.
 intros. destruct H; dcr; subst.
 eexists x; split; eauto.
-eapply drop_get. orewrite (k + (n - k) = n); eauto.
+eapply get_app_ge; eauto.
 Defined.
 
 
@@ -418,10 +316,10 @@ Lemma renestSim_sim r L L' E s n D L'' ZL
             get ZL f Z /\
             approx L' Z (drop (f - block_n b) D) f' b b')
       (DEF:labelsDefined s (length D))
-      (SIM:renILabenv bisim_progeq r PR (zip pair ZL D) L L')
+      (SIM:simILabenv Bisim r PR (zip pair ZL D) L L')
       (DROP:drop n L' = mapi_impl I.mkBlock n (snd (egalize D n s)) ++ L'')
       (LEN1:length L = length D) (LEN2:length L = length ZL)
-  : bisim'r r (L, E, s) (L', E, fst (egalize D n s)).
+  : sim'r r Bisim (L, E, s) (L', E, fst (egalize D n s)).
 Proof.
   revert_except s.
   sind s; intros; destruct s; simpl in *; invt labelsDefined;
@@ -440,20 +338,13 @@ Proof.
   - edestruct SIM as [SIM1 SIM2].
     edestruct (get_in_range D H2) as [f' GetD].
     edestruct SL as [b [b' [Z ?]]]; eauto; dcr; eauto. invt approx.
-    destruct l as [f]; simpl in *.
     repeat let_case_eq; repeat let_pair_case_eq; simpl in * |- *; subst.
     decide (length Z = length Y).
     + case_eq (omap (exp_eval E) Y); [ intros | intros; pno_step; eauto ].
-      exploit SIM2; eauto using zip_get.
-      simpl. orewrite (f' + 0 = f'). eauto.
-      simpl in *. inv H8. unfold progeq in H22. simpl in *. unfold bisim'r.
-      destruct H21; dcr; subst. inv_get. inv SIM. dcr.
-      exploit (sawtooth_smaller H17 H0); eauto.
-      simpl in *. assert (f_eq: f = f - n0 + n0) by omega. rewrite <- f_eq in *.
-      repeat get_functional.
-      erewrite get_nth; eauto using zip_get.
-      eapply bisim_drop_shift_left; eauto. simpl.
-      eapply H22; eauto with len.
+      exploit (SIM2 l (LabI f')); eauto using zip_get.
+      simpl in *. dcr; subst.
+      erewrite get_nth; [| eauto].
+      eapply H10; try eassumption. eauto with len.
     + pno_step; simpl in *.
       erewrite get_nth in Ldef; eauto. get_functional. eauto.
   - pno_step.
@@ -461,7 +352,7 @@ Proof.
     pextern_step.
     + left. eapply IH; eauto.
     + left. eapply IH; eauto.
-  - rename s into F. eapply bisim'_expansion_closed;
+  - rename s into F. eapply sim'_expansion_closed;
                        [ | eapply star2_silent; [ econstructor | eapply star2_refl ]
                          | eapply star2_refl].
     assert (SL': forall f f' : nat,
@@ -501,13 +392,15 @@ Proof.
         rewrite map_length; eauto.
         rewrite mapi_length. eauto.
     }
-    eapply IH; eauto.
+    eapply IH; eauto with len.
     + rewrite app_length, mapi_length; eauto.
     + rewrite zip_app; eauto with len.
-      eapply renILabenv_extension; eauto 10 with len.
-      intros ? ? ? ? ? ? ? ? GetF RN GetL' GetA. simpl. inv_get.
-      destruct RN as [? [? ?]]; subst. simpl.
-      rewrite get_app_lt in H; eauto 20 using get_range with len.
+      eapply simILabenv_extension; eauto 10 with len.
+      intros.
+      intros ? ? ? ? ? ? ? ? RN GetF GetL' GetA. simpl.
+      inv_get. simpl in *; dcr; subst.
+      destruct RN; dcr. subst.
+      rewrite get_app_lt in H2; eauto 20 using get_range with len.
       inv_get; simpl in *. unfold plus' in GetL'.
       eapply drop_get in GetL'.
       rewrite DROP in GetL'. repeat rewrite mapi_app in GetL'.
@@ -517,13 +410,9 @@ Proof.
       inv_get. clear EQ.
       destruct x as [Z' s']; simpl.
       destruct (egalize_funs_get _ _ GetF GetL'); eauto; subst.
-      split; [|eauto].
-      split; [ hnf; eauto|].
-      intros ? ? ? ? ? [? [B ?]] SIM'; subst; simpl in *.
-      rewrite <- zip_app in SIM'.
       edestruct (@egalize_funs_get2 (mapi (plus' n) F ++ D) (❬F❭ + n) F) as [LX EQ]; eauto;
         simpl in *.
-      eapply IH; eauto. simpl in *.
+      eapply IH; eauto with len. simpl in *.
       * rewrite app_length, mapi_length. exploit H1; eauto.
       * instantiate (1:=LX).
         rewrite <- egalize_funs_length2.
@@ -536,9 +425,18 @@ Proof.
         rewrite egalize_funs_length1 in DROP.
         rewrite drop_drop in DROP.
         rewrite DROP. f_equal. f_equal. rewrite plus_comm. eauto.
-      * eauto with len.
-      * eauto with len.
-      * eauto with len.
+      * hnf; intros. simpl.
+        inv_get. simpl. destruct H; dcr.
+        rewrite get_app_lt in H4; eauto 20 using get_range with len.
+        inv_get. simpl in *. unfold plus' in H2.
+        eapply drop_get in H2.
+        rewrite DROP in H2. repeat rewrite mapi_app in H2.
+        repeat rewrite <- app_assoc in H2.
+        rewrite get_app_lt in H2;
+          [| rewrite mapi_impl_length, egalize_funs_length1; eauto 20 using get_range].
+        inv_get. clear EQ.
+        destruct x as [Z' s']; simpl.
+        destruct (egalize_funs_get _ _ H0 H2); eauto; subst. eauto.
     + rewrite <- egalize_funs_length2 at 1. simpl.
       repeat rewrite mapi_app in DROP.
       repeat rewrite <- app_assoc in DROP.
@@ -549,6 +447,4 @@ Proof.
       repeat rewrite drop_drop in DROP. simpl. rewrite Plus.plus_assoc.
       rewrite DROP. simpl.
       rewrite <- egalize_funs_length2. f_equal. f_equal. omega.
-    + eauto with len.
-    + eauto with len.
 Qed.
