Coherence/Allocation.v
@@ -762,29 +762,6 @@ Qed.
 
 (** ** local injectivity only looks at variables occuring in the program *)
 
-Lemma incl_minus_incl_union X `{OrderedType X} s t u
-  : s \ t ⊆ u
-    -> s ⊆ t ∪ u.
-Proof.
-  intros. rewrite <- H0. cset_tac.
-Qed.
-
-Lemma incl_union_lr_eq X `{OrderedType X} s t u v
-  : s ∪ t [=] u
-    -> v ∪ t ⊆ v ∪ u.
-Proof.
-  intros. rewrite <- H0. eauto with cset.
-Qed.
-
-Lemma incl_add_union_union X `{OrderedType X} s x t u
-  : s [=] {x; t}
-    -> {x; u} ∪ t ⊆ u ∪ s.
-Proof.
-  intros. rewrite H0. cset_tac.
-Qed.
-
-Hint Immediate incl_minus_incl_union incl_union_lr_eq incl_add_union_union : cset.
-
 Lemma locally_inj_live_agree s ϱ ϱ' ara alv ZL Lv
       (LS:live_sound FunctionalAndImperative ZL Lv s alv)
       (sd: renamedApart s ara)
